A lot more cleanup

symexec.dfy
@@ -1,29 +1,4 @@
-//Todo:
-//Figure out tree representation with Michael's queue stuff.
-//Figure out following classes/modules/etc.:
-//    State: how we represent variable value assignemnts here will
-//        affect how we implement PC.
-//    Scheduler: need to manage tree, add and pop functions, reason
-//        about state exploration.
-//    PC: need to figure out how to represent and call external
-//        SAT solver.
-//    exec module: come up with an interface for (sybolic) instruction
-//        execution.
 
-//We need to define State, it should have: PC, variables, variables to
-//values mapping, instructions, and a function to get the next instruction.
-
-//We need to build the scheduler.  It needs to do bookkeeping and build a tree
-//about which we can prove the properties from the king paper.
-
-//PC is a boolean expression over symbolic inputs (values).  Need to have
-//update functions for this to be used in exec.  The important thing with
-//PC is that we can give it to a SAT solver.  Assuming we want this to run code
-//beyond a proof, that means calling a solver from dafny, and ensuring the PC
-//conforms to the solver's interface.
-
-//include "Dpll.dfy"
-//include "PropLogic.dfy"
 include "sat.dfy"
 include "scheduler.dfy"
 include "executor.dfy"
@@ -37,12 +12,36 @@ method Main()
   scheduler.printTree();
 }
 
-// Path conditions in leaf nodes do not overlap.
-// That is, any assignment of variables leads to exactly one leaf node.
-predicate king2(scheduler: TreeQueue)
+// King Property 1
+// All nodes in the tree should be satisfyable.
+//
+// Verification: This property is simple to verify since we explicitly don't
+// enqueue to the scheduler if the path condition is not satisfyable. We
+// simply added this as a loop invariant in the main loop.
+predicate king1(scheduler: Scheduler)
   requires scheduler != null
   requires scheduler.a != null
-  reads scheduler, scheduler.a
+  reads *
+{
+  forall i :: 0 <= i < scheduler.a.Length ==> match scheduler.a[i]
+    case Some(node) => node != null && SatLib.sat(node.pc)
+    case None => true
+}
+
+// King Property 2
+// Path conditions in leaf nodes do not overlap.
+// That is, any assignment of variables leads to exactly one leaf node.
+//
+// Verification: "step_execution()" and "Scheduler.Enqueue()" have the major
+// proof obligations. "Scheduler.Enqueue()" requires and ensures king2, but it
+// has some preconditions needed to prove this, namely that the input nodes
+// don't have overlapping pc's with any other leaves (except parent) and the
+// two input nodes don't overlap with each other. "step_execution()" must prove
+// that these preconditions hold. It does so using basic boolean axioms that
+// are assumed by the sat interface (see sat.dfy).
+predicate king2(scheduler: Scheduler)
+  requires scheduler != null
+  requires scheduler.a != null
   reads *
 {
   forall i,j :: 0 <= i < scheduler.a.Length && 0 <= j < scheduler.a.Length ==>
@@ -59,49 +58,31 @@ predicate king2(scheduler: TreeQueue)
 // The core of the symbolic execution engine. Explore state in the order
 // according to the scheduler, ensuring that a state is only explored if
 // it can be reached (the path condition leading to it is satisfyable).
-method symex() returns (scheduler: TreeQueue)
-  decreases *  // Possibly non-terminating
+method symex() returns (scheduler: Scheduler)
+  decreases *
   ensures scheduler != null
   ensures scheduler.a != null
-
-  // King Property 1
-  // All nodes in the tree should be satisfyable.
-  //
-  // Verification: This property is simple to verify since we explicitly don't
-  // enqueue to the scheduler if the path condition is not satisfyable. We
-  // simply added this as a loop invariant in the main loop.
-  ensures forall i :: 0 <= i < scheduler.a.Length ==> match scheduler.a[i]
-    case Some(node) => node != null && SatLib.sat(node.pc)
-    case None => true;
-
-  // King Property 2
   ensures scheduler.a.Length >= 1
-  ensures king2(scheduler)
 
+  ensures king1(scheduler)
+  ensures king2(scheduler)
 {
   var initState := getInitialState();
-  scheduler := new TreeQueue(initState);
+  scheduler := new Scheduler(initState);
 
   assert !scheduler.isEmpty();
   while !scheduler.isEmpty()
-    decreases *  // Possibly non-terminating
+    decreases *
     invariant scheduler.a != null
     invariant scheduler.Valid()
 
-    // Nodes are always satisfyable (else they are not enqueued)
-    // Used to verify King Prop 1
-    invariant forall i :: 0 <= i < scheduler.a.Length ==> match scheduler.a[i]
-      case Some(node) => node != null && SatLib.sat(node.pc)
-      case None => true;
-
-    // Used to verify King Prop 2
+    invariant king1(scheduler)
     invariant king2(scheduler)
-    //invariant 2*scheduler.start+2 >= scheduler.end
 
   {
-    var state_node := scheduler.Dequeue();
-    if state_node != null {
-      step_execution(scheduler, state_node);
+    var node := scheduler.Dequeue();
+    if node != null {
+      step_execution(scheduler, node);
     }
 
   }
@@ -111,11 +92,10 @@ method symex() returns (scheduler: TreeQueue)
 
 // Enqueue the children of state_node, but only if their path condition
 // is satisfyable.
-method step_execution(scheduler: TreeQueue, state_node: Node)
+method step_execution(scheduler: Scheduler, state_node: Node)
   requires scheduler != null
   requires scheduler.a != null
   requires state_node != null
-  requires SatLib.sat(state_node.pc)
   requires scheduler.Valid() && scheduler.start >= 0
   requires scheduler.a[scheduler.start].Some?
   requires scheduler.a[scheduler.start].v == state_node
@@ -124,12 +104,9 @@ method step_execution(scheduler: TreeQueue, state_node: Node)
   ensures scheduler.Valid()
 
   // Used for King 1
-  requires forall i :: 0 <= i < scheduler.a.Length ==> match scheduler.a[i]
-    case Some(node) => node != null && SatLib.sat(node.pc)
-    case None => true;
-  ensures forall i :: 0 <= i < scheduler.a.Length ==> match scheduler.a[i]
-    case Some(node) => node != null && SatLib.sat(node.pc)
-    case None => true;
+  requires king1(scheduler)
+  ensures king1(scheduler)
+  requires SatLib.sat(state_node.pc)
 
   // Used for King 2
   requires king2(scheduler)
@@ -148,9 +125,6 @@ method step_execution(scheduler: TreeQueue, state_node: Node)
   var s1_pc := SatLib.and(state_node.pc, bc);
   var s2_pc := SatLib.and(state_node.pc, SatLib.not(bc));
 
-  // Used for King 1
-  assert !SatLib.sat(SatLib.and(s1_pc, s2_pc));
-
   // state_node satisfies King 2
   // This is exactly like King 2, except node_j is always the last dequeue'd
   // node.
@@ -163,22 +137,11 @@ method step_execution(scheduler: TreeQueue, state_node: Node)
       !SatLib.sat(SatLib.and(node_i.pc, node_j.pc))
     );
 
-  // Intermediate assertion that helps prove the next one.
-  assert forall i :: 0 <= i < scheduler.a.Length ==>
-    var node_i := match scheduler.a[i] case Some(node) => node case None => null;
-    var node_j := match scheduler.a[scheduler.start] case Some(node) => node case None => null;
-    node_i != null && node_j != null && i != scheduler.start &&
-    isLeaf(i, scheduler.a)
-    ==> (
-      (!SatLib.sat(SatLib.and(SatLib.and(node_i.pc, node_j.pc), bc))) &&
-      (!SatLib.sat(SatLib.and(node_i.pc, SatLib.and(node_j.pc, bc)))) &&
-      (!SatLib.sat(SatLib.and(SatLib.and(node_i.pc, node_j.pc), SatLib.not(bc)))) &&
-      (!SatLib.sat(SatLib.and(node_i.pc, SatLib.and(node_j.pc, SatLib.not(bc)))))
-    );
-
   // Path conditions for the nodes we are about to enqueue do not overlap with
   // any existing leaves, except the parent node.
   // Final precondition we need before Enqueue.
+  // Uses: Associativity of "and"
+  // Uses: Zero Axiom of "and"
   assert forall i :: 0 <= i < scheduler.a.Length ==>
     var node_i := match scheduler.a[i] case Some(node) => node case None => null;
     node_i != null && i != scheduler.start &&
@@ -190,8 +153,6 @@ method step_execution(scheduler: TreeQueue, state_node: Node)
 
   var node1: Node := null;
   var node2: Node := null;
-  var node1_maybe: NodeMaybe := NodeMaybe.None;
-  var node2_maybe: NodeMaybe := NodeMaybe.None;
   if !SatLib.sat(s1_pc) {
 
     // Used for King 2
@@ -199,39 +160,21 @@ method step_execution(scheduler: TreeQueue, state_node: Node)
     assert SatLib.sat(s2_pc);
 
     node2 := new Node(s2_state, s2_pc);
-    node1_maybe, node2_maybe := scheduler.Enqueue(null, node2);
+    scheduler.Enqueue(null, node2);
   } else if !SatLib.sat(s2_pc) {
     node1 := new Node(s1_state, s1_pc);
-    node1_maybe, node2_maybe := scheduler.Enqueue(node1, null);
+    scheduler.Enqueue(node1, null);
   } else {
     node1 := new Node(s1_state, s1_pc);
     node2 := new Node(s2_state, s2_pc);
 
     // Used for King 2
-    assert !SatLib.sat(SatLib.and(s1_pc, s2_pc));
+    // Uses: Communativity of "and"
+    // Uses: Associativity of "and"
+    // Uses: Negation Axiom of "and"
+    // Uses: Zero Axiom of "and"
     assert !SatLib.sat(SatLib.and(node1.pc, node2.pc));
 
-    node1_maybe, node2_maybe := scheduler.Enqueue(node1, node2);
+    scheduler.Enqueue(node1, node2);
   }
 }
-
-/*
-module SAT_Func{
-import opened dpll : DPLL
-import opened PropLogic
-
-method SAT(formula: Formula) returns (sat_bool: bool)
-decreases *
-{
-var alpha : Option<Assignment> := dpll.DPLL(formula);
-
- var temp_sat_bool := false;
-  if !(alpha == Option<Assignment>.None){
-   temp_sat_bool := true;
-  }
-sat_bool := temp_sat_bool;
-}
-
-}
-*/
-
